instanciar trie como container

Trie.fst
@@ -3,20 +3,17 @@ module Trie
 open FStar.Vector
 module U32 = FStar.UInt32
 module U = FStar.UInt
-
-let alphabet_size : U32.t = U32.uint_to_t 26
-
-// b_nat represents a bounded natural that can fit in 32 bits
-type b_nat = x:nat{x < U32.v alphabet_size /\ U.size x 32}
-
-noeq
-type trie0 (n : U32.t) =
-  | L
-  | N of raw (trie0 n) n & bool
+open TrieDataType
+open FStar.Classical.Sugar
+open Container
 
 type trie_array = raw (trie0 alphabet_size) alphabet_size
 
 let empty : trie0 alphabet_size = L
+
+// ==========================
+//  Trie Operations
+// ==========================
 
 let rec mem (l : list b_nat) (t : trie0 alphabet_size) : Tot bool (decreases l) =
   match t with
@@ -66,3 +63,307 @@ let rec delete0 (l: list b_nat) (t : trie0 alphabet_size) : Tot (trie0 alphabet_
                   then L
                   else N (a',b')
         | t'' -> N (update a (U32.uint_to_t x) t'', is_t)
+
+// ==========================
+//  Operations Lemmas
+// ==========================
+
+// ---- insert Lemma ----
+
+let rec insert0_trie (l:list b_nat) (t:trie0 alphabet_size)
+  : Lemma (requires is_trie t) (ensures is_trie (insert0 l t))
+  =
+  match (t,l) with
+  | (L,[]) -> ()
+  | (_,[]) -> ()
+  | (L,x::xs) -> insert0_trie xs L
+  | (N (a, b), x::xs) -> insert0_trie xs (index a (U32.uint_to_t x))
+
+let insert (x:list b_nat) (t:trie) : trie
+  =
+  insert0_trie x t;
+  insert0 x t
+
+// ---- is_empty Lemma ----
+
+// -- exists child node ==> not (is_empty a) --
+
+let rec del_lem_back2 (a:trie_array)
+                      (i':b_nat)
+                      (pf:squash (not (is_empty' a i')))
+  : Tot (squash (not (is_empty a))) (decreases (U32.v alphabet_size - i'))
+  =
+  if i' = U32.v alphabet_size - 1
+  then pf
+  else let pf' : squash (not (is_empty' a (i'+1))) = () in
+       del_lem_back2 a (i'+1) pf'
+
+let del_lem_back1 (a:trie_array)
+  : Lemma (requires (exists (i:b_nat).
+                     N? (index a (U32.uint_to_t i))))
+          (ensures not (is_empty a))
+  =
+  let pf : squash (exists (i': b_nat). not (is_empty' a i')) = () in
+  exists_elim
+  #_
+  #(fun i' -> not (is_empty' a i'))
+  #(not (is_empty a))
+  pf
+  (del_lem_back2 a)
+
+let del_lem_back (a:trie_array)
+  : Lemma ((exists (i:b_nat).
+                    N? (index a (U32.uint_to_t i)))
+           ==>
+          (not (is_empty a)))
+  =
+  implies_intro (exists (i:b_nat).
+                         N? (index a (U32.uint_to_t i)))
+                (fun pfp -> (not (is_empty a)))
+                (fun pfp -> del_lem_back1 a)
+
+// -- exists child node <== not (is_empty a) --
+
+let rec del_lem' (a:trie_array) (i:b_nat)
+  : Lemma (requires not (is_empty' a i))
+          (ensures (exists (i:b_nat).
+                            N? (index a (U32.uint_to_t i))))
+  =
+  if N? (index a (U32.uint_to_t i))
+  then ()
+  else if i = 0
+      then ()
+      else del_lem' a (i-1)
+
+let del_lem (a:trie_array)
+  : Lemma (requires not (is_empty a))
+          (ensures (exists (i:b_nat).
+                            N? (index a (U32.uint_to_t i))))
+  = del_lem' a (U32.v alphabet_size - 1)
+
+// ---- delete Lemma ----
+
+let rec delete0_trie (l:list b_nat) (t:trie0 alphabet_size)
+  : Lemma (requires is_trie t) (ensures is_trie (delete0 l t))
+  =
+  match (t,l) with
+  | (L,_) -> ()
+  | (N (a,_), []) -> if is_empty a then () else del_lem a
+  | (N (a,is_t), x::xs) ->
+      match index a (U32.uint_to_t x) with
+      | L -> ()
+      | t' ->
+        match delete0 xs t' with
+        | L -> let N (a',b') = N (update a (U32.uint_to_t x) L , is_t)
+               in if is_empty a' && not is_t
+                  then ()
+                  else if is_t then () else del_lem a'
+        | t'' -> delete0_trie xs t'
+
+let delete (x:list b_nat) (t:trie) : trie
+  =
+  delete0_trie x t;
+  delete0 x t
+
+// ==========================
+//  Tries as containers
+// ==========================
+
+let models
+  (xs : trie0 alphabet_size)
+  (ss : TSet.set (list b_nat))
+  : GTot prop
+  =
+  forall (x: list b_nat).
+         mem x xs <==> TSet.mem x ss
+
+let empty_ok_lem (_:unit) : Lemma (models empty TSet.empty)
+  = ()
+
+let rec is_empty_lem (t:trie{N? t})
+  : squash (exists (l:list b_nat) . mem l t) 
+  =
+  match t with
+  | N (a,true) -> assert(mem [] t)
+  | N (a,false) ->
+    let pf : squash (exists (i:b_nat).
+                             N? (index a (U32.uint_to_t i))) = ()
+    in exists_elim
+       #b_nat
+       #(fun i -> N? (index a (U32.uint_to_t i)))
+       #(exists (l:list b_nat) . mem l t)
+       pf
+       (fun i pfx -> (
+                      is_empty_lem (index a (U32.uint_to_t i));
+                      assert(exists (l:list b_nat). mem (i::l) t)
+                      )
+       )
+
+let is_empty_ok (xs:trie)
+  : Lemma (models xs TSet.empty <==> L? xs)
+  =
+  match xs with
+  | L -> ()
+  | N (_,_) -> is_empty_lem xs
+
+let rec mem_insert (t:trie) (l: list b_nat)
+  : Lemma (mem l (insert l t))
+  =
+  match (t,l) with
+  | (_,[]) -> ()
+  | (L, x::xs) -> mem_insert t xs
+  | (N (a,is_t), x::xs) -> mem_insert (index a (U32.uint_to_t x)) xs
+
+let rec ins_ok_lem1 (t:trie) (l: list b_nat) (l':(list b_nat){mem l' t})
+  : Tot (squash (mem l' (insert l t))) (decreases l')
+  =
+  match (t,l,l') with
+  | (_,_,[]) -> ()
+  | (_,[],_) -> ()
+  | (L,_,_) -> ()
+  | (N (a,b), x::xs, y::ys) ->
+    if x = y
+    then (
+          match index a (U32.uint_to_t x) with
+          | L -> ()
+          | t' -> ins_ok_lem1 t' xs ys
+         )
+    else ()
+
+let rec ins_ok_lem2 (t:trie) (l: list b_nat) (l':(list b_nat){not (mem l' t) /\ (l <> l')})
+  : Tot (squash (not (mem l' (insert l t)))) (decreases l')
+  =
+  match (t,l,l') with
+  | (_,_,[]) -> ()
+  | (_,[],_) -> ()
+  | (L, x::xs, y::ys) ->
+    if x = y then ins_ok_lem2 L xs ys else ()
+  | (N (a, b), x::xs, y::ys) ->
+    if x = y
+    then ins_ok_lem2 (index a (U32.uint_to_t x)) xs ys
+    else ()
+
+let ins_ok_lem (x:list b_nat) (xs:trie) (ss : TSet.set (list b_nat))
+  : Lemma (requires xs `models` ss)
+          (ensures  insert x xs
+                     `models`
+                    TSet.union ss (TSet.singleton x))
+  =
+  mem_insert xs x;
+
+  forall_intro (l:(list b_nat){mem l xs})
+               (fun l' -> mem l' (insert x xs))
+               (ins_ok_lem1 xs x);
+
+  forall_intro (l:(list b_nat){not (mem l xs) /\ (l <> x)})
+               (fun l' -> not (mem l' (insert x xs)))
+               (ins_ok_lem2 xs x)
+
+let rec mem_delete (t:trie) (l:list b_nat)
+  : Lemma (not (mem l (delete l t)))
+  =
+  match (t,l) with
+  | (L,_) -> ()
+  | (_,[]) -> ()
+  | (N (a,b), x::xs) ->
+      match index a (U32.uint_to_t x) with
+      | L -> ()
+      | t' ->
+        match delete0 xs t' with
+        | L -> ()
+        | t'' -> mem_delete t' xs
+
+let rec del_ok_lem1 (t:trie) (l:list b_nat) (l':(list b_nat){not (mem l' t)})
+  : Tot (squash (not (mem l' (delete l t))))
+  =
+  match (t,l,l') with
+  | (L,_,_) -> ()
+  | (N(_,_),_,[]) -> ()
+  | (N(_,_),[],_) -> ()
+  | (N (a,_), x::xs, y::ys) -> 
+    if x = y
+    then (
+          match index a (U32.uint_to_t x) with
+          | L -> ()
+          | t' ->
+            match delete0 xs t' with
+            | L -> ()
+            | t'' -> del_ok_lem1 t' xs ys
+         )
+    else ()
+
+let del_ok_lem2' (t:trie{N? t}) (l:(list b_nat){Cons? l})
+  : Lemma (requires (let N (a,_) = t in is_empty a))
+          (ensures not (mem l t))
+  =
+  match (t,l) with
+  | (N (a,_),_) -> del_lem_back a
+
+let rec del_ok_lem2 (t:trie) (l:list b_nat) (l':(list b_nat){(mem l' t) /\ (l <> l')})
+  : Tot (squash (mem l' (delete l t)))
+  =
+  match (t,l,l') with
+  | (L,_,_) -> ()
+  | (N(_,_),_,[]) -> ()
+
+  | (N(a,_),[],x::xs) ->
+    if is_empty a
+    then del_ok_lem2' t l'
+    else ()
+
+  | (N (a, is_t), x::xs, y::ys) -> 
+    if x = y
+    then (
+          match index a (U32.uint_to_t x) with
+          | L -> ()
+          | t' -> del_ok_lem2 t' xs ys
+         )
+    else (
+          match index a (U32.uint_to_t x) with
+          | L -> ()
+          | t' -> del_lem_back (update a (U32.uint_to_t x) L)
+         )
+
+let del_ok_lem (x:list b_nat) (t:trie) (ss: TSet.set (list b_nat))
+  : Lemma (requires t `models` ss)
+          (ensures delete x t
+                   `models`
+                   TSet.intersect ss (TSet.complement <| TSet.singleton x))
+  =
+  mem_delete t x;
+
+  //assume(forall (l:(list b_nat){not (mem t l)}). not (mem (delete x t) l));
+  forall_intro (l:(list b_nat){not (mem l t)})
+               (fun l' -> not (mem l' (delete x t)))
+               (del_ok_lem1 t x);
+  
+  //assume(forall (l:(list b_nat){(mem t l) /\ (l <> x)}). (mem (delete x t) l));
+  forall_intro (l:(list b_nat){(mem l t) /\ (l <> x)})
+               (fun l' -> mem l' (delete x t))
+               (del_ok_lem2 t x)
+
+instance tries_are_containers0
+  : container0 (list b_nat) trie = {
+    empty = L;
+    is_empty = L?;
+
+    mem = mem;
+    ins = insert;
+    del = delete;
+  }
+
+instance tries_are_container_laws
+  : container_laws (list b_nat) trie tries_are_containers0 = {
+    models = models;
+    empty_ok = empty_ok_lem;
+    is_empty_ok = is_empty_ok;
+    mem_ok = (fun _ _ _ -> ());
+    ins_ok = ins_ok_lem;
+    del_ok = del_ok_lem;
+}
+
+instance tries_are_containers
+  : container (list b_nat) trie = {
+    ops = tries_are_containers0;
+    laws = tries_are_container_laws;
+  }
