Client.Indexed.fst
@@ -1,0 +1,27 @@
+module Client.Indexed
+
+open Container.Indexed
+open TrieDataType
+open Trie
+
+let l1 : list b_nat = [1]
+let l2 : list b_nat = [1;2]
+let l3 : list b_nat = [1;2;3]
+let l4 : list b_nat = [4]
+
+let test #s {| icontainer (list b_nat) s |} () =
+  let e : s _ = empty in
+  let e = ins l1 e in
+  let e = ins l2 e in
+  let e = ins l3 e in
+  let e = ins l4 e in
+  let e = del l2 e in
+  assert (mem l1 e);
+  assert (not (mem l2 e));
+  assert (mem l3 e);
+  assert (mem l4 e);
+  ()
+
+let test_list () =
+  test #_ #(icontainer_from_container (list b_nat) trie
+               FStar.Tactics.Typeclasses.solve) ()
