Trie.fsti
@@ -1,0 +1,13 @@
+module Trie
+
+open Container
+open TrieDataType
+
+instance val tries_are_containers0
+  : container0 (list b_nat) trie
+
+instance val tries_are_container_laws
+  : container_laws (list b_nat) trie tries_are_containers0
+
+instance val tries_are_containers
+  : container (list b_nat) trie
