TrieDataType.fst
@@ -1,0 +1,40 @@
+module TrieDataType
+
+open FStar.Vector
+module U32 = FStar.UInt32
+module U = FStar.UInt
+
+let alphabet_size : U32.t = U32.uint_to_t 26
+
+// b_nat represents a bounded natural that can fit in 32 bits
+type b_nat = x:nat{x < U32.v alphabet_size /\ U.size x 32}
+
+let functio (b_nat) : bool = true
+
+let v : b_nat = 25
+
+noeq
+type trie0 (n : U32.t) =
+  | L
+  | N of raw (trie0 n) n & bool
+
+let index_dec (#a:Type) (l:len_t) (v:raw a l) (i : U32.t{U32.v i < U32.v l})
+  : Lemma (index v i << v)
+          [SMTPat (index v i)]
+  = admit()
+
+let rec is_trie (t:trie0 alphabet_size) : Tot prop
+  =
+  match t with
+  | L -> true
+  | N (a,true) ->
+    (forall (i:b_nat).
+      is_trie (index a (U32.uint_to_t i)))
+  | N (a,false) ->
+    (forall (i:b_nat).
+      is_trie (index a (U32.uint_to_t i)))
+    /\
+    (exists (i:b_nat).
+        N? (index a (U32.uint_to_t i)))
+
+type trie = t:(trie0 alphabet_size){is_trie t}
